src/tests/tmDefinition.v
@@ -1,8 +1,19 @@
 
 (* From ASUB Require Import core. *)
 
+Definition foo := (fun {A:Type} (x: A) => x).
+Compute foo 1.
+
+(* while the above with foo works, below does not.
+ So even though we can specify implicit variables in constr_expr, Coq seems to just use this info
+ if we are in a Definition. The kernel AST econstr does not carry this information anymore.
+ Depending on what tmUnquote does (run_template_monad.ml suggests that it is translated to econstr) we could not even add
+ implicit arguments to metacoq lambdas *)
+Fail Compute ((fun {A:Type} (x: A) => x) 1).
+
 From MetaCoq.Template Require Import utils All.
 Import ListNotations MonadNotation Nat.
+
 
 Module tests.
   Definition congr_test :=
@@ -30,11 +41,10 @@ Module tests.
   Definition oneisonetest : TemplateMonad unit :=
     (* one_q <- tmQuote 1;; *)
     (* eq_q <- tmQuote eq;; *)
-    (* eq_refl_q <- tmQuote Logic.eq_refl;; *)
     (* typ <- tmUnquote (Ast.tApp eq_q [one_q; one_q]);; *)
     (* typ' <- tmEval lazy (typ.(my_projT2));; *)
     (* a.d. todo, we can't explicitly give types to our definitions? *)
-    obj <- tmDefinitionRed "oneisone_q" (Some lazy) (@Logic.eq_refl _ 1);;
+    obj <- tmDefinitionRed "oneisone_q" (Some lazy)  (@Logic.eq_refl _ 1);;
     tmReturn tt.
                  
   MetaCoq Run oneisonetest.
@@ -44,7 +54,7 @@ Module tests.
 
   (* Same definition but with a term unquoted by MetaCoq *)
   Definition oneisonetest2 : TemplateMonad unit :=
-    one_q <- tmQuote 1;;
+    (* one_q <- tmQuote 1;; *)
     (* eq_refl_q <- tmQuote eq_refl;; *)
     (* tm <- tmUnquote (Ast.tApp eq_refl_q [Ast.hole; one_q]);; *)
     tm <- tmUnquote eq_refl_q;;
@@ -64,15 +74,24 @@ Module tests.
     obj <- tmDefinitionRed "oneisone_q3" (Some lazy) tm;;
     tmReturn obj.
 
+  MetaCoq Quote Definition zero_q := 0.
   (* this fails when I use hole instead of nat because MetaCoq apparently cannot unquote evars? *)
-  Definition oneisonetest3 : TemplateMonad unit :=
+  Definition oneisonetest3 : TemplateMonad unit.
+  Proof.
+    refine (
     one_q <- tmQuote 1;;
-    nat_q <- tmQuote nat;;
-    (* tm <- tmUnquote (Ast.tApp eq_refl_q [Ast.hole; one_q]);; *)
+    nat_q <- tmQuote nat;; _).
+    (* a.d. ok so apparently I can use holes when I state beforehand the gallina term to which it should conform. But that is probably not usable in my code. *)
+    assert (H: 0 = 0). {
+    let x := eval cbv in (Ast.tApp eq_refl_q [Ast.hole; zero_q ]) in
+        denote_term x (fun k => exact k).
+    }
+    refine (
     tm <- tmUnquote (Ast.tApp eq_refl_q [nat_q; one_q]);;
     tm <- tmEval lazy (my_projT2 tm);;
     obj <- tmDefinitionRed "oneisone_q3" (Some lazy) tm;;
-    tmReturn tt.
+    tmReturn tt).
+  Defined.
 
   MetaCoq Run oneisonetest3.
   Check oneisone_q3.
@@ -80,33 +99,177 @@ Module tests.
   MetaCoq Quote Definition tru := True.
   MetaCoq Quote Definition i := I.
 
-  Set Printing All.
-  Fail Definition oneisonetest3 : TemplateMonad unit :=
-  (@bind TemplateMonad TemplateMonad_Monad typed_term unit (tmUnquote tru)
-     (fun typ : typed_term =>
-      @bind TemplateMonad TemplateMonad_Monad (my_projT1 typ) unit (@tmEval all (my_projT1 typ) (my_projT2 typ))
-        (fun typ0 : (my_projT1 typ) =>
-         @bind TemplateMonad TemplateMonad_Monad typed_term unit (tmUnquote i)
-           (fun proof : typed_term =>
-            @bind TemplateMonad TemplateMonad_Monad (my_projT1 proof) unit
-              (@tmEval all (my_projT1 proof) (my_projT2 proof))
-              (fun proof0 : (my_projT1 proof) =>
-               @bind TemplateMonad TemplateMonad_Monad (my_projT1 typ) unit
-                 (@tmDefinitionRed "oneisone4" (Some lazy) typ0 proof0)
-                 (fun _ : _ => @tmReturn unit tt)))))).
-                 
+  (* Set Printing All. *)
+  (* wenn ich nach dem (fun ty: Type) versuche es in dem bind oder tmEval zu benutzen funktioniert es leider nicht, da statisch keine Verbindung zwischen my_projT1 t und ty existiert. *)
   Definition oneisonetest4 : TemplateMonad unit :=
-    proof <- tmUnquote i;;
-    t <- tmEval lazy (my_projT1 proof);;
-    t' <- tmEval lazy (my_projT2 proof);;
-    tmPrint t;;
-    tmPrint t';;
+  (@bind TemplateMonad TemplateMonad_Monad typed_term unit (tmUnquote i)
+     (fun t : typed_term =>
+      @bind TemplateMonad TemplateMonad_Monad Type unit (@tmEval all Type (my_projT1 t))
+            (fun ty : Type =>
+             @bind TemplateMonad TemplateMonad_Monad (my_projT1 t) unit (@tmEval all (my_projT1 t) (my_projT2 t))
+                   (fun tm : (my_projT1 t) =>
+                    @bind TemplateMonad TemplateMonad_Monad (my_projT1 t) unit
+                          (@tmDefinitionRed "oneisone4" (Some lazy) (my_projT1 t) tm)
+                          (fun _ : _ => @tmReturn unit tt))))).
+                 
+  MetaCoq Run oneisonetest4.
+  Check oneisone4.
+
+  (*** Finally this works. Just use tmUnquoteTyped to assign the type of the proof then we can use the same type in tmDefinition *)
+  (* MetaCoq Quote Definition id_q := (fun x:Set => x). *)
+  
+  Definition oneisonetest5 : TemplateMonad unit :=
+    (* let tru' := tApp id_q [tru] in *)
+    ty <- tmUnquoteTyped Type tru;;
+    proof <- tmUnquoteTyped ty i;;
+    @tmDefinitionRed "oneisone5" (Some lazy) ty proof;;
     tmReturn tt.
 
-  MetaCoq Run oneisonetest4.
+  MetaCoq Run oneisonetest5.
+  Print oneisone5.
+  (* Unset Printing All. *)
+
+  Definition oneisonetest6: TemplateMonad unit :=
+    proof <- tmUnquote i;;
+    ty <- tmEval all (my_projT1 proof);;
+    tm <- tmEval all (my_projT2 proof);;
+    tmPrint ty;;
+    tmPrint (my_projT1 proof);;
+    obj <- @tmDefinitionRed "oneisone_q6" (Some (unfold (Common_kn "my_projT1"))) (my_projT1 proof) tm;;
+    (* obj <- tmDefinitionRed "oneisone_q6" None tm;; *)
+    (* obj <- tmEval all obj;; *)
+    tmReturn tt.
+
+  MetaCoq Run oneisonetest6.
+  (* Compute (my_projT1 (existT_typed_term True I)). *)
+  Check oneisone_q6.
 
   (* a.d. todo, quote definition with implicits *)
   Definition myid {A:Type} (a:A) := a.
-  Fail MetaCoq Quote Definition myid_source := Eval compute in myid.
+  (* Fail MetaCoq Quote Definition myid_source := Eval compute in myid. *)
   (* Print myid_source. *)
 
+  (* define a fixpoint *)
+  Fixpoint add (n m : nat) :=
+    match n return _ with
+    | O => m
+    | S n => S (add n m)
+    end.
+
+
+  MetaCoq Quote Definition add_source := Eval compute in add.
+  Print add_source.
+  MetaCoq Test Quote add.
+
+  Fixpoint even (n:nat) :=
+    match n with
+    | O => true
+    | S n => odd n
+    end
+  with odd n :=
+    match n with
+    | O => false
+    | S n => even n
+    end.
+
+  Compute even 4.
+  Compute even 5.
+  Compute odd 4.
+  Compute odd 5.
+
+  Inductive foo : nat -> Type :=
+  | foo0 : forall n, foo n
+  | foo1 : nat -> foo 0.
+   Fixpoint bla (n: nat) (d: foo n) :=
+    match d with
+    | foo0 _ => false
+    | foo1 _ => true
+    end.
+
+  MetaCoq Test Quote odd.
+
+  MetaCoq Quote Definition even_source := Eval compute in even.
+  MetaCoq Quote Definition odd_source := Eval compute in odd.
+  MetaCoq Quote Definition bla_source := Eval compute in bla.
+  Print even_source.
+  (* the second argument to tFix is an index into the list of mutual fixpoint definitions *)
+  Print odd_source.
+  Print bla_source.
+
+  Definition tmTypedDefinition (lem: string * term * term) : TemplateMonad unit :=
+    let '(name, typ_q, t_q) := lem in
+    typ <- tmUnquoteTyped Type typ_q;;
+    t <- tmUnquoteTyped typ t_q;;
+    @tmDefinitionRed name (Some TemplateMonad.Common.all) typ t;;
+    tmReturn tt.
+
+  (* ok so I can just use a hole for the type here *)
+  MetaCoq Run (tmTypedDefinition ("even2", hole, even_source)).
+  MetaCoq Run (tmTypedDefinition ("odd2", hole, odd_source)).
+
+  Compute even2 4.
+  Compute even2 5.
+  Compute odd2 4.
+  Compute odd2 5.
+
+
+
+  MetaCoq Quote Definition nat_q := nat.
+  
+ Definition myfix : term := tFix
+  [{|
+     dname :=
+       {| binder_name := nNamed "myadd"; binder_relevance := Relevant |};
+     dtype :=
+       tProd
+         {| binder_name := nNamed "n"; binder_relevance := Relevant |}
+         nat_q
+         (tProd
+          {| binder_name := nNamed "m"; binder_relevance := Relevant |}
+          nat_q
+          nat_q);
+     dbody :=
+       tLambda
+         {| binder_name := nNamed "n"; binder_relevance := Relevant |}
+         nat_q
+         (tLambda
+            {| binder_name := nNamed "m"; binder_relevance := Relevant |}
+            nat_q
+            (tCase
+               ({|
+                   inductive_mind :=
+                     (MPfile ["Datatypes"; "Init"; "Coq"], "nat");
+                   inductive_ind := 0
+                 |}, 0, Relevant)
+               (tLambda
+                  {| binder_name := nNamed "n"; binder_relevance := Relevant |}
+                  nat_q
+                  nat_q)
+               (tRel 1)
+               (* the first component of the pair seems to be the number of arguments of the constructor *)
+               [(0, (tRel 0));
+               (1,
+                tLambda
+                  {|
+                    binder_name := nNamed "n"; binder_relevance := Relevant
+                  |}
+                  (tInd
+                     {|
+                       inductive_mind :=
+                         (MPfile ["Datatypes"; "Init"; "Coq"], "nat");
+                       inductive_ind := 0
+                     |} []) (tApp <% S %> [tApp (tRel 3) [tRel 0; tRel 1]]))]));
+     rarg := 0
+   |}] 0.
+
+ MetaCoq Unquote Definition myfix' := myfix.
+ Compute (myfix' 4 5).
+
+ MetaCoq Run (tmUnquoteTyped (list nat) (tApp <% @nil %> [hole]) >>= tmPrint).
+ Definition foo2 X (x y:X) := x.
+
+ (* wow so it actually works if we specify the type with tmUnquoteTyped
+  * but since we also compute the type for the tmUnquoteTyped call we actually need another tmUnquoteTyped before *)
+ MetaCoq Run (
+           tmUnquoteTyped Type <% bool %> >>= fun nat_uq =>
+           tmUnquoteTyped nat_uq (tApp <% foo2 %> [hole; <% true %>; <% false %>]) >>= tmPrint).
