listimport/importfile1.v
@@ -1,0 +1,5 @@
+Require Import List.
+
+Goal forall P, P -> P.
+  easy.
+Qed.
