listimport/importfile2.v
@@ -1,0 +1,7 @@
+From ASUB Require Import importfile1.
+
+(* ssreflect rewrite due to List import is transitive *)
+Goal forall P Q, P <-> Q -> P -> Q.
+Proof.
+  intros P Q H. rewrite H. easy.
+Qed.
