listimport/localimport1.v
@@ -1,0 +1,9 @@
+Require List. 
+
+Module proofs.
+
+  Goal forall P Q, P <-> Q -> P -> Q.
+    intros P Q H. rewrite H. easy.
+  Qed.
+
+End proofs.
