listimport/samefile.v
@@ -1,0 +1,11 @@
+Goal forall P Q, P <-> Q -> P -> Q.
+Proof.
+  intros P Q H. Fail rewrite H.
+Abort.
+
+Require Import List.
+
+Goal forall P Q, P <-> Q -> P -> Q.
+Proof.
+  intros P Q H. rewrite H. easy.
+Qed.
