src/AssocList.v
@@ -1,0 +1,238 @@
+Require Import List String.
+Import ListNotations.
+#[ local ]
+Open Scope string.
+
+Require Import Arith.
+From ASUB Require Import Utils.
+
+Module Type Discrete.
+  Parameter t : Set.
+  Parameter eqb : t -> t -> bool.
+End Discrete.
+
+Module String_Discrete.
+  Definition t := string.
+  Definition eqb := String.eqb.
+End String_Discrete.
+
+(* Module bla : Discrete := String_Discrete.  *)
+
+(* My own implementation of string as ordered type. Mainly tried it to improve performance when
+ the example in Graph.v did not run anymore. Turns out that was because I changed size_ind in Utils.v to
+ Qed. instead of Defined.
+ But keeping it now since it's probably faster than the stdlib implementation that first converts
+ the ascii to binary nats *)
+(* Module MyStringOT. *)
+(*   Definition t := string. *)
+(*   (* Definition cmp := String_as_OT.cmp. *) *)
+  
+(*   Compute (match " ", "#" with *)
+(*            | String a_head _, String b_head _ => *)
+(*              Ascii_as_OT.cmp a_head b_head *)
+(*            | _, _ => Eq *)
+(*            end). *)
+  
+(*   Definition Ascii_cmp (a b : Ascii.ascii) : comparison := *)
+(*     match a, b with *)
+(*       (* least significant bit is on the left *) *)
+(*     | Ascii.Ascii a0 a1 a2 a3 a4 a5 a6 a7, Ascii.Ascii b0 b1 b2 b3 b4 b5 b6 b7 => *)
+(*       match Bool.compare a7 b7 with *)
+(*       | Eq => *)
+(*         match Bool.compare a6 b6 with *)
+(*         | Eq => *)
+(*           match Bool.compare a5 b5 with *)
+(*           | Eq => *)
+(*             match Bool.compare a4 b4 with *)
+(*             | Eq => *)
+(*               match Bool.compare a3 b3 with *)
+(*               | Eq => *)
+(*                 match Bool.compare a2 b2 with *)
+(*                 | Eq => *)
+(*                   match Bool.compare a1 b1 with *)
+(*                   | Eq => *)
+(*                     Bool.compare a0 b0 *)
+(*                   | x => x *)
+(*                   end *)
+(*                 | x => x *)
+(*                 end *)
+(*               | x => x *)
+(*               end *)
+(*             | x => x *)
+(*             end *)
+(*           | x => x *)
+(*           end *)
+(*         | x => x *)
+(*         end *)
+(*       | x => x *)
+(*       end *)
+(*     end. *)
+
+(*   (* Compute (match " " with *) *)
+(*   (*          | String head _ => *) *)
+(*   (*            head *) *)
+(*   (*          | "" => Ascii.Ascii false false false false false false false false *) *)
+(*   (*          end). *) *)
+(*   (* Compute (match "c", "b" with *) *)
+(*   (*          | String a_head _, String b_head _ => *) *)
+(*   (*            Ascii_cmp a_head b_head *) *)
+(*   (*          | _, _ => Eq *) *)
+(*   (*          end). *) *)
+  
+(*   Fixpoint cmp (a b : t) : comparison := *)
+(*     match a with *)
+(*     | "" => match b with *)
+(*            | "" => Eq *)
+(*            | String _ _ => Lt *)
+(*            end *)
+(*     | String a_head a_tail => *)
+(*       match b with *)
+(*       | "" => Gt *)
+(*       | String b_head b_tail => *)
+(*         match Ascii_cmp a_head b_head with *)
+(*         | Eq => cmp a_tail b_tail *)
+(*         | Lt => Lt *)
+(*         | Gt => Gt *)
+(*         end *)
+(*       end *)
+(*     end. *)
+
+(*   (* Compute (cmp "Hello" "Hella"). *) *)
+
+(* End MyStringOT.  *)
+
+
+(* DONE use more naive implementation that does not have ordering invariant
+ * surprisingly this might even have better performance because our lists are very small in most cases *)
+Module FMap (X: Discrete).
+  (* Finite maps represented as association lists.
+   * Invariant: keys are unique *)
+
+  Definition key := X.t.
+  Definition t (elt: Type) := list (key * elt)%type.
+
+  Definition empty {elt: Type} : t elt := [].
+
+  Fixpoint add {elt: Type} (s: t elt) (k: key) (v: elt) : t elt :=
+    match s with
+    | [] => [(k, v)]
+    | (k', v') :: s' =>
+      if X.eqb k k'
+      then (k, v) :: s'
+      else (k', v') :: (add s' k v)
+    end.
+
+  Fixpoint union {elt: Type} (s0 s1: t elt) : t elt :=
+    match s0 with
+    | [] => s1
+    | (k, v) :: s0' =>
+      union s0' (add s1 k v)
+    end.
+  
+  Fixpoint mem {elt: Type} (s: t elt) (k: key) : bool :=
+    match s with
+    | [] => false
+    | (k', _) :: s' =>
+      if X.eqb k k'
+      then true
+      else mem s' k
+    end.
+
+  Fixpoint find {elt: Type} (s: t elt) (k: key) : option elt :=
+    match s with
+    | [] => None
+    | (k', v) :: s' =>
+      if X.eqb k k'
+      then Some v
+      else find s' k
+    end.
+
+  Fixpoint fold {elt A: Type} (f: key -> elt -> A -> A) (s: t elt) (state: A) : A :=
+    match s with
+    | [] => state
+    | (k, v) :: s' => fold f s' (f k v state)
+    end.
+
+  Fixpoint map {elt elt': Type} (f: elt -> elt') (s: t elt) : t elt' :=
+    match s with
+    | [] => []
+    | (k, v) :: s' => (k, f v) :: map f s'
+    end.
+
+  Fixpoint mapi {elt elt': Type} (f: key -> elt -> elt') (s: t elt) : t elt' :=
+    match s with
+    | [] => []
+    | (k, v) :: s' => (k, f k v) :: mapi f s'
+    end.
+    
+  (* a.d. todo, no guarantees about overwriting. I'm using elements -> List.map -> fromList to replace mapi since mapi seems bugged *)
+  Fixpoint fromList {elt : Type} (A: list (key * elt)) : t elt :=
+    match A with
+    | [] => []
+    | (k, v) :: A' => add (fromList A') k v
+    end.
+  
+End FMap. 
+
+(* Module SFMap := FMap MyStringOT. *)
+Module SFMap := FMap String_Discrete.
+
+Module FSet (X: Discrete).
+
+  Definition elt := X.t.
+  Definition t := list elt.
+
+  Definition empty : t := [].
+
+  Definition elements (s: t) : list elt := s.
+
+  Definition singleton (v: elt) : t := [v].
+
+  Fixpoint mem (s: t) (v: elt) :=
+    match s with
+    | [] => false
+    | v' :: s' =>
+      if X.eqb v v'
+      then true
+      else mem s' v
+    end.
+
+  Fixpoint add (s: t) (v: elt) :=
+    match s with
+    | [] => [v]
+    | v' :: s' =>
+      if X.eqb v v'
+      then v' :: s'
+      else v' :: (add s' v)
+    end.
+
+  Fixpoint fromList (l: list elt) :=
+    match l with
+    | [] => empty
+    | v :: l =>
+      add (fromList l) v
+    end.
+
+  Fixpoint union (s0 s1: t) : t :=
+    match s0 with
+    | [] => s1
+    | v :: s0' =>
+      union s0' (add s1 v)
+    end.
+
+  (* Lemma intersection (s0 s1: t) : t. *)
+End FSet.
+
+(* Module SSet := FSet MyStringOT. *)
+Module SSet := FSet String_Discrete.
+  
+
+
+
+
+
+
+
+
+
+           
