src/DeBruijnMap.v
@@ -1,0 +1,27 @@
+Require Import String List.
+Import ListNotations.
+
+Module DB.
+  Definition t := string -> option nat.
+  
+  Definition empty : t := fun _ => None.
+
+  Definition shift (dbmap: t) : t :=
+    fun s' =>
+      match dbmap s' with
+      | None => None
+      | Some n => Some (S n)
+      end.
+
+  Definition add (s: string) (dbmap: t) : t :=
+    fun s' =>
+      if eqb s s' then Some 0
+      else shift dbmap s'.
+
+  Fixpoint adds (ss: list string) (dbmap: t) : t :=
+    match ss with
+    | [] => dbmap
+    | s :: ss =>
+      adds ss (add s dbmap)
+    end.
+End DB.
