src/ErrorM.v
@@ -1,0 +1,20 @@
+Require Import String.
+Open Scope string.
+
+From ASUB Require Import Monad.
+
+(* a.d. TODO maybe write the error monad directly. *)
+
+(* Adding the module type annotation breaks other modules because then E is not transparent
+ * TODO find out why *)
+Module EArgs (* : RWSEParams *).
+  Definition R := unit.
+  Definition W := unit.
+  Definition S := unit.
+  Definition E := string.
+
+  Definition append := fun (_ _: unit) => tt.
+  Definition empty := tt.
+End EArgs.
+
+Module ErrorM := RWSE EArgs.
