src/GallinaGen.v
@@ -1,0 +1,148 @@
+From MetaCoq.Template Require Import All.
+Require Import String List.
+From ASUB Require Import GenM AssocList DeBruijnMap.
+
+(* TODO add another node for embedded terms. This should be a bit more performant when we use predefined terms like "eq" since we don't really need to look them up in the environment. *)
+Inductive nterm : Type :=
+| nRef : string -> nterm (* turns into tRel, tConst, tInd, tConstruct from the normal term type *)
+| nHole : nterm
+| nTerm : term -> nterm
+| nProd : string -> nterm -> nterm -> nterm
+| nArr : nterm -> nterm -> nterm
+| nLambda : string -> nterm -> nterm -> nterm
+| nApp : nterm -> list nterm -> nterm
+| nFix : mfixpoint nterm -> nat -> nterm
+| nCase : string -> nat -> nterm -> nterm -> list (nat * nterm) -> nterm.
+
+
+Fixpoint mknArr (nt0: nterm) (nts: list nterm) :=
+  match nts with
+  | [] => nt0
+  | nt :: nts =>
+    nArr nt0 (mknArr nt nts)
+  end.
+
+Fixpoint mknArrRev (nts: list nterm) (nt0: nterm) :=
+  match nts with
+  | [] => nt0
+  | nt :: nts => nArr nt (mknArrRev nts nt0)
+  end.
+
+Import GenM.Notations GenM.
+
+(* MetaCoq Test Quote (match 1 with O => O | S x => x end). *)
+
+(*
+Import MonadNotation.
+MetaCoq Run (let tm := (tCase
+                          (* the type of the discriminant *)
+     ({| inductive_mind := (MPfile ["Datatypes"; "Init"; "Coq"]%list, "nat"); inductive_ind := 0 |}, 0,
+      Relevant)
+     (tLambda {| binder_name := nNamed "x"; binder_relevance := Relevant |}
+              (* (tInd {| inductive_mind := (MPfile ["Datatypes"; "Init"; "Coq"]%list, "nat"); inductive_ind := 0 |} *)
+              (*       []%list) *)
+              (* (tInd {| inductive_mind := (MPfile ["Datatypes"; "Init"; "Coq"]%list, "nat"); inductive_ind := 0 |} *)
+              (*       []%list)) *)
+              hole hole)
+     (tApp
+        (tConstruct
+           {| inductive_mind := (MPfile ["Datatypes"; "Init"; "Coq"]%list, "nat"); inductive_ind := 0 |} 1
+           []%list)
+        [tConstruct
+           {| inductive_mind := (MPfile ["Datatypes"; "Init"; "Coq"]%list, "nat"); inductive_ind := 0 |} 0
+           []%list])
+     [(0,
+       tConstruct {| inductive_mind := (MPfile ["Datatypes"; "Init"; "Coq"]%list, "nat"); inductive_ind := 0 |} 0
+                  []%list);
+     (1,
+      tLambda {| binder_name := nNamed "x"; binder_relevance := Relevant |}
+              (* (tInd {| inductive_mind := (MPfile ["Datatypes"; "Init"; "Coq"]%list, "nat"); inductive_ind := 0 |} *)
+              (*       []%list) *) hole (tRel 0))]) in
+              tmUnquoteTyped nat tm >>= tmPrint).
+ *)
+
+(* TODO maybe make it option string but then I don't have error handling.
+ * Just a possible performance improvement *)
+Definition get_fix_name (d: def nterm) : GenM.t string :=
+  match binder_name (dname d) with
+  | nAnon => error "Fixpoint without a name."
+  | nNamed s => pure s
+  end.
+
+(* TODO already defined somewhere? *)
+Definition get_inductive (s: string) : GenM.t inductive :=
+  env <- asks snd;;
+  match SFMap.find env s with
+  | None => error (append "get_inductive: not found: " s)
+  | Some t => match t with
+             | tInd ind _ => pure ind
+             | _ => error "wrong kind of term"
+             end
+  end.
+    
+Fixpoint translate (dbmap: DB.t) (t: nterm) : GenM.t term :=
+  match t with
+  | nRef s =>
+    (* check dbmap and environment *)
+    match dbmap s with
+    | Some n => pure (tRel n)
+    | None =>
+      env <- asks snd;;
+      match SFMap.find env s with
+      | Some t => pure t
+      | None => error (append "Unknown Identifier during Gallina Translation: " s)
+      end
+    end
+  | nHole => pure hole
+  | nTerm t => pure t
+  | nProd s nt0 nt1 =>
+    let n := {| binder_name := nNamed s; binder_relevance := Relevant |} in
+    t0 <- translate dbmap nt0;;
+    (* add the newly bound variable when translating nt1 *)
+    let dbmap' := DB.add s dbmap in
+    t1 <- translate dbmap' nt1;;
+    pure (tProd n t0 t1)
+  | nArr nt0 nt1 =>
+    let n := {| binder_name := nAnon; binder_relevance := Relevant |} in
+    t0 <- translate dbmap nt0;;
+    (* just shift the dbmap when translating nt1 *)
+    let dbmap' := DB.shift dbmap in
+    t1 <- translate dbmap' nt1;;
+    pure (tProd n t0 t1)
+  | nLambda s nt0 nt1 =>
+    let n := {| binder_name := nNamed s; binder_relevance := Relevant |} in
+    t0 <- translate dbmap nt0;;
+    (* add the newly bound variable when translating nt1 *)
+    let dbmap' := DB.add s dbmap in
+    t1 <- translate dbmap' nt1;;
+    pure (tLambda n t0 t1)
+  | nApp nt nts =>
+    t <- translate dbmap nt;;
+    ts <- a_map (translate dbmap) nts;;
+    pure (tApp t ts)
+  | nFix mfixs n =>
+    fixNames <- a_map get_fix_name mfixs;;
+    let dbmap' := DB.adds fixNames dbmap in
+    mfixs <- a_map (fun '{| dname := nname; dtype := ntype; dbody := nbody; rarg := nrarg |} =>
+                     ttype <- translate dbmap ntype;;
+                     (* the fixpoint names are only bound in the bodies *)
+                     tbody <- translate dbmap' nbody;;
+                     pure {| dname := nname; dtype := ttype; dbody := tbody; rarg := nrarg |})
+                  mfixs;;
+    pure (tFix mfixs n)
+  | nCase indName paramNum nelimPred ndiscr nbranches =>
+    telimPred <- translate dbmap nelimPred;;
+    tdiscr <- translate dbmap ndiscr;;
+    tbranches <- a_map (fun '(n, nt) =>
+                         t <- translate dbmap nt;;
+                         pure (n, t))
+                      nbranches;;
+    ind <- get_inductive indName;;
+    pure (tCase (ind, paramNum, Relevant) telimPred tdiscr tbranches)
+  end.
+
+Definition translate_lemma (l: GenM.t (string * nterm * nterm)) : GenM.t (string * term * term) :=
+  '(lname, ntype, nbody) <- l;;
+  ttype <- translate DB.empty ntype;;
+  tbody <- translate DB.empty nbody;;
+  pure (lname, ttype, tbody).
