src/GenM.v
@@ -1,0 +1,109 @@
+Require Import String List.
+Import ListNotations.
+Open Scope string.
+
+From MetaCoq.Template Require Import All.
+Import MonadNotation.
+From ASUB Require Import Monad Language AssocList Utils TemplateMonadUtils Quotes.
+
+Record State := { st_names : list string }.
+
+Definition empty_state := {| st_names := [] |}.
+(* Definition initial_env := SFMap.fromList [("nat", nat_q); ("eq", eq_q); ("f_equal", f_equal_q); ("eq_refl", eq_refl_q); ("eq_trans", eq_trans_q); ("up_ren", up_ren_q); ("funcomp", funcomp_q); ("var_zero", var_zero_q); ("scons", scons_q); ("id", id_q); ("shift", shift_q); ("ap", ap_q); ("up_ren_ren", up_ren_ren_q)]. *)
+Definition initial_env := SFMap.fromList [("nat", nat_q)].
+
+Definition update_env (env env' : SFMap.t term) : SFMap.t term :=
+  SFMap.union env env'.
+
+Definition tm_update_env '{| st_names := names; |} (env: SFMap.t term) : TemplateMonad (SFMap.t term) :=
+  env_list' <- tm_mapM locate_name names;;
+  let env' := SFMap.fromList env_list' in
+  tmReturn (update_env env' env). 
+  
+
+(* The RWSE monad that we use to generate the lemmas *)
+Module GenMArgs.
+  Definition R := (Signature * (SFMap.t term))%type.
+  Definition W := string.
+  Definition S := State.
+  Definition E := string.
+
+  Definition append := String.append.
+  Definition empty := ""%string.
+End GenMArgs.
+
+Module GenM.
+  Module GenM := RWSE GenMArgs.
+  Include GenM.
+
+  Import Notations.
+
+  Definition register_name (name: string) : t unit :=
+    '{| st_names := names |} <- get;;
+    put {| st_names := name :: names |}.
+
+  Definition register_names (names': list string) : t unit :=
+    '{| st_names := names |} <- get;;
+    put {| st_names := app names' names |}.
+
+  (* Definition env_get (s: string) : t term := *)
+  (*   env <- gets st_env;; *)
+  (*   match SFMap.find env s with *)
+  (*   | None => error (String.append "Not found: " s) *)
+  (*   | Some t => pure t *)
+  (*   end. *)
+
+  Definition testrun {A} (mv: t A) :=
+    run mv (Hsig_example.mySig, initial_env) empty_state.
+
+  (** * Additional functions used during code generation *)
+
+  (** get the constructors of a sort *)
+  Definition constructors (sort: tId) : t (list Constructor) :=
+    spec <- asks (fun x => sigSpec (fst x));;
+    match SFMap.find spec sort with
+    | Some cs => pure cs
+    | None => error ("constructors called with unknown sort")
+    end.
+
+  (** get the arguments of a sort *)
+  Definition getArguments (sort: tId) : t (list tId) :=
+    args <- asks (fun x => sigArguments (fst x));;
+    match SFMap.find args sort with
+    | Some sorts => pure sorts
+    | None => error ("getArguments called with unknown sort")
+    end.
+
+  (** check if a sort has renamings *)
+  Definition hasRenaming (sort: tId) : t bool :=
+    rens <- asks (fun x => sigRenamings (fst x));;
+    pure (SSet.mem rens sort).
+
+  (** return the substitution vector for a sort *)
+  Definition substOf (sort: tId) : t (list tId) :=
+    substs <- asks (fun x => sigSubstOf (fst x));;
+    match SFMap.find substs sort with
+    | Some sorts => pure sorts
+    | None => error ("substOf called with unknown sort")
+    end.
+
+  (** check if a sort is open (has a variable constructor) *)
+  Definition isOpen (sort: tId) : t bool :=
+    isOpen <- asks (fun x => sigIsOpen (fst x));;
+    pure (SSet.mem isOpen sort).
+
+  (** A sort is definable if it has any constructor *)
+  Definition isDefinable (sort: tId) : t bool :=
+    b <- isOpen sort;;
+    ctors <- constructors sort;;
+    pure (orb b (negb (list_empty ctors))).
+
+  (** Check if the arguments of the first sort of a component and the component itself overlaps
+   ** We can only check the first element of the component because they all have the same
+   ** substitution vector. *)
+  Definition isRecursive (component: NEList.t tId) : t bool :=
+    let '(sort, _) := component in
+    args <- getArguments sort;;
+    pure (negb (list_empty (list_intersection (NEList.to_list component) args))).
+  
+End GenM.
