src/NEList.v
@@ -1,0 +1,32 @@
+Require Import List.
+Import ListNotations.
+
+From ASUB Require Import Utils.
+
+Definition t (A: Type) := (A * list A)%type.
+
+Definition hd {A: Type} (ne: t A) : A :=
+  let '(v, l) := ne in v.
+
+Definition tl {A: Type} (ne: t A) : list A :=
+  let '(v, l) := ne in l.
+
+Definition to_list {A: Type} (ne: t A) : list A :=
+  let '(v, l) := ne in
+  v :: l.
+
+Definition from_list {A: Type} (l: list A) : option (t A) :=
+  match l with
+  | [] => None
+  | a :: l => Some (a, l)
+  end.
+
+Definition map {A B: Type} (f: A -> B) (ne: t A) : t B :=
+  let '(x, l) := ne in
+  (f x, List.map f l).
+
+Definition fold_left {A B: Type} (f: A -> B -> A) (ne: t B) (init: A) : A :=
+  List.fold_left f (to_list ne) init.
+
+Definition anyf {A: Type} (f: A -> bool) (ne: t A) : bool :=
+  list_anyf f (to_list ne).
