src/Names.v
@@ -1,0 +1,14 @@
+Require Import String List.
+Import ListNotations.
+Open Scope string.
+
+Definition separator := "_".
+Definition sep x y := x ++ separator ++ y.
+Fixpoint sepd xs :=
+  match xs with
+  | [] => ""
+  | [x] => x
+  | x :: xs => sep x (sepd xs)
+  end.
+
+Definition varConstrName x := sep "var" x.
