src/Quotes.v
@@ -1,0 +1,19 @@
+From MetaCoq.Template Require Import All.
+From ASUB Require Import core unscoped.
+
+MetaCoq Quote Definition nat_q := nat.
+MetaCoq Quote Definition eq_q := @eq.
+MetaCoq Quote Definition eq_trans_q := @eq_trans.
+MetaCoq Quote Definition eq_sym_q := @eq_sym.
+MetaCoq Quote Definition eq_refl_q := @eq_refl.
+MetaCoq Quote Definition f_equal_q := @f_equal.
+MetaCoq Quote Definition up_ren_q := up_ren.
+MetaCoq Quote Definition funcomp_q := @funcomp.
+MetaCoq Quote Definition var_zero_q := var_zero.
+MetaCoq Quote Definition scons_q := @scons.
+MetaCoq Quote Definition id_q := @id.
+MetaCoq Quote Definition shift_q := shift.
+MetaCoq Quote Definition ap_q := @ap.
+MetaCoq Quote Definition up_ren_ren_q := @up_ren_ren.
+
+  
