src/SigAnalyzer.v
@@ -1,0 +1,143 @@
+Require Import List String.
+Import ListNotations.
+Open Scope string.
+
+From ASUB Require Import Language Graph AssocList Monad Utils ErrorM.
+From ASUB Require NEList.
+Import ErrorM.Notations ErrorM.
+
+Module G := Digraph.
+
+(** * Build a graph where the vertices are all the sorts from the spec and there
+ ** * is an edge u->v iff v occurs directly in u (i.e. if there is some constructor
+ ** * of u where v is an argument head. ) *)
+Definition build_graph (spec: Spec) :=
+  SFMap.fold (fun sort ctors g0 =>
+                let args := flat_map getArgs ctors in
+                fold_left (fun g1 arg => G.add_edge g1 sort arg)
+                          args g0)
+             spec G.empty.
+
+
+Definition binder_analysis (spec: Spec) (occurs_in: G.vertex -> G.vertex -> bool) : ErrorM.t SSet.t :=
+  SFMap.fold (fun sort ctors mbs0 =>
+                let positions := flat_map con_positions ctors in
+                fold_left (fun mbs1 '{| pos_binders := pos_binders; pos_head := pos_head |} =>
+                             let binders := flat_map getBinders pos_binders in
+                             fold_left (fun mbs2 bound_sort =>
+                                          bs <- mbs2;;
+                                          let vacuous := list_nonef (fun arg => occurs_in arg bound_sort) (getArgSorts pos_head) in
+                                          if vacuous
+                                          then error "vacuous!"
+                                          else pure (SSet.add bs bound_sort))
+                                       binders mbs1
+                          )
+                          positions mbs0)
+             spec (ErrorM.pure SSet.empty).
+
+
+(** * A sort needs renamings
+ ** * either if it appears in a constructor in the same component
+ ** * or if it occurs in a sort that needs renamings *)
+Definition renaming_analysis (spec: Spec) (g_trans: G.t) (components: list (NEList.t tId)) : SSet.t :=
+  let renamings := SSet.empty in
+  (* add all sorts to the set that appear in their component *)
+  let renamings := fold_left (fun ren0 (component: NEList.t tId) =>
+                                let boundSorts := getBoundSorts spec component in
+                                let has_bound := NEList.anyf (fun sort => list_mem sort boundSorts) component in
+                                if has_bound
+                                then SSet.union ren0 (SSet.fromList (NEList.to_list component))
+                                else ren0)
+                             components renamings in
+  (* then go through all sorts and add those that occur in sorts already in the set *)
+  G.fold g_trans (fun sort adj ren0 =>
+                    if SSet.mem ren0 sort 
+                    then SSet.union ren0 adj
+                    else ren0)
+         renamings.
+
+(** * The substitution vector of a sort consist of the open sorts that occur in it. *)
+Definition subordination (g: G.t) (canonical_order: list tId) (open_sorts: SSet.t) : tId -> list tId :=
+  fun sort => filter (fun subst_sort =>
+                     (SSet.mem open_sorts subst_sort
+                      && G.mem_edge g sort subst_sort)%bool)
+                  canonical_order.
+
+(** Calculate the strongly connected components *)
+(* TODO using a hack here to convert the non-empty list to a normal list temporarily
+ * but it should be possible to implement the sorting if if I have a proof that the canonical_order list contains all sorts. (maybe even declare a finite string type indexed by this canonical_order) *)
+Definition topological_sort g (canonical_order: list tId) : list (NEList.t tId) :=
+  list_filter_map (fun component => NEList.from_list (list_intersection canonical_order (NEList.to_list component))) (G.scc_list g).
+
+Definition build_signature (componentsO: option (list (NEList.t tId))) (canonical_order: list tId) (spec: Spec) : ErrorM.t Signature :=
+  let g := build_graph spec in
+  open_sorts <- binder_analysis spec (G.mem_edge (G.transitive_closure g false));;
+  let substs := subordination (G.transitive_closure g true) canonical_order open_sorts in
+  let subst_of := SFMap.mapi (fun sort _ => substs sort) spec in
+  let components := match componentsO with None => topological_sort g canonical_order | Some c => c end in
+  let arguments := SFMap.mapi (fun sort _ => match G.succ g sort with None => [] | Some x => x end) spec in
+  (* let arguments := SFMap.fromList (map (fun '(sort, _) => (sort, match G.succ g sort with None => [] | Some x => x end)) (SFMap.elements spec)) in *)
+  let renamings := renaming_analysis spec (G.transitive_closure g false) components in
+  pure {| sigSpec := spec;
+          sigSubstOf := subst_of;
+          sigComponents := components;
+          sigIsOpen := open_sorts;
+          sigArguments := arguments;
+          sigRenamings := renamings
+       |}.
+
+
+Module Ex.
+  Definition spec := Hsig_example.mySigSpec.
+  Definition g := build_graph spec.
+  Open Scope string.
+
+  Compute g.
+  Compute (G.invert g).
+
+  (* test occurs_in relation *)
+  Compute bool_beq (G.mem_edge g "ty" "ty") true.
+  Compute bool_beq (G.mem_edge g "ty" "tm") false.
+  Compute bool_beq (G.mem_edge g "ty" "vl") false.
+  Compute bool_beq (G.mem_edge g "tm" "ty") true.
+  Compute bool_beq (G.mem_edge g "tm" "tm") true.
+  Compute bool_beq (G.mem_edge g "tm" "vl") true.
+  Compute bool_beq (G.mem_edge g "vl" "ty") true.
+  Compute bool_beq (G.mem_edge g "vl" "tm") true.
+  Compute bool_beq (G.mem_edge g "vl" "vl") false.
+
+  (* test open sorts *)
+  Definition open_sorts := (match run (binder_analysis spec (G.mem_edge (G.transitive_closure g false))) tt tt with
+                            | inl _ => SSet.empty
+                            | inr (_, _, x) => x
+                            end).
+  Compute open_sorts.
+
+  Definition substs := subordination (G.transitive_closure g true) ["ty"; "tm"; "vl"] open_sorts.
+  (* While it does not diverge it takes a very long time to compute. This and the trouble with the actually diverging function call above indicates that I should write my own finmaps *)
+  Compute (SFMap.mapi (fun sort _ => substs sort) spec).
+  (* Compute (SFMap.fromList (map (fun '(sort, _) => (sort, substs sort)) (SFMap.elements spec))). *)
+
+  Compute (run (build_signature (Some [("ty", []); ("tm", ["vl"])]) ["ty"; "tm"; "vl"] spec) tt tt).
+  Compute (run (build_signature None ["ty"; "tm"; "vl"] spec) tt tt).
+  Compute (G.succ g "ty").
+  Compute (G.succ g "tm").
+  Compute (G.succ g "vl").
+
+  Definition components := [("tm", ["vl"]); ("ty", [])].
+  Compute (renaming_analysis spec (G.transitive_closure (G.invert g) false) components).
+
+End Ex.
+
+Module Ex2.
+  Definition spec := Hsig_fol.mySigSpec.
+  Definition g := build_graph spec.
+  Open Scope string.
+
+  Compute g.
+  Definition components : list (NEList.t tId) := [("form", []); ("term", [])].
+  (* as expected this is the empty list *)
+  Compute (renaming_analysis spec (G.transitive_closure (G.invert g) false) components).
+
+  Compute (run (build_signature None ["term"; "form"] spec) tt tt).
+End Ex2.
