src/TemplateMonadUtils.v
@@ -1,0 +1,54 @@
+From MetaCoq.Template Require Import All Pretty.
+Require Import List String.
+Import ListNotations MonadNotation.
+
+Fixpoint tm_sequence {A: Type} (mvals: list (TemplateMonad A)) : TemplateMonad (list A) :=
+  match mvals with
+  | [] => tmReturn []
+  | mval :: mvals =>
+    val <- mval;;
+    vals <- tm_sequence mvals;;
+    tmReturn (val :: vals)
+  end.
+
+Fixpoint tm_mapM {A B: Type} (f: A -> TemplateMonad B) (l: list A) : TemplateMonad (list B) :=
+  match l with
+  | [] => tmReturn []
+  | a :: l =>
+    b <- f a;;
+    bs <- tm_mapM f l;;
+    tmReturn (b :: bs)
+  end.
+
+Fixpoint tm_foldM {A B: Type} (f: A -> B -> TemplateMonad A) (l: list B) (init: A) : TemplateMonad A :=
+  match l with
+  | [] => tmReturn init
+  | b :: l =>
+    init <- f init b;;
+    tm_foldM f l init
+  end.
+
+(** * Register a definition in the Coq environment given the quoted representation of its type and term.
+ ** * This works with terms that contain holes (but the types must not, else Coq cannot infer all holes) *)
+Definition tmTypedDefinition (lem: string * term * term) : TemplateMonad unit :=
+  let '(name, typ_q, t_q) := lem in
+  typ <- tmUnquoteTyped Type typ_q;;
+  t <- tmUnquoteTyped typ t_q;;
+  @tmDefinitionRed name (Some TemplateMonad.Common.hnf) typ t;;
+  tmReturn tt.
+
+(* MetaCoq Run (tmTypedDefinition "mynatnil" <% list nat %> (tApp <% @nil %> [hole])). *)
+          
+Definition locate_name (name: string) : TemplateMonad (string * term) :=
+  loc <- tmLocate1 name;;
+  match loc with
+  | IndRef ind => tmReturn (name, tInd ind [])
+  | ConstructRef ind n => tmReturn (name, tConstruct ind n [])
+  | ConstRef kn => tmReturn (name, tConst kn [])
+  | _ => tmFail (String.append "unknown name or name is not an inductive/constructor/constant: " name)
+  end.
+
+(* kind of works but it's not completely evaluated *)
+Definition my_print_term (t: term) : TemplateMonad unit :=
+  let s := print_term ([], Monomorphic_ctx (LevelSet.Mkt [], ConstraintSet.Mkt [])) [] false t in
+  tmEval TemplateMonad.Common.all s >>= tmPrint.
