src/Termutil.v
@@ -1,0 +1,71 @@
+Require Import String Arith List.
+Import ListNotations.
+
+From ASUB Require Import Language Utils Quotes GallinaGen.
+From MetaCoq.Template Require Import Ast.
+
+Open Scope string.
+
+Definition nat_ := nTerm nat_q.
+Definition eq_ (s t: nterm) := nApp (nTerm eq_q) [nHole; s; t].
+Definition eq_refl_ := nApp (nTerm eq_refl_q) [nHole; nHole].
+Definition ap_ (s t: nterm) := nApp (nTerm ap_q) [ nHole; nHole; s; nHole; nHole; t ].
+Definition eq_trans_ (s t: nterm) := nApp (nTerm eq_trans_q) [nHole; nHole; nHole; nHole; s; t].
+Definition eq_sym_ (s: nterm) := nApp (nTerm eq_sym_q) [nHole; nHole; nHole; s].
+Definition f_equal_ (feq_lam s t H: nterm) := nApp (nTerm f_equal_q) [nHole; nHole; feq_lam; s; t; H].
+Definition up_ren_ (s: nterm) := nApp (nTerm up_ren_q) [s].
+Definition scons_ (s t: nterm) := nApp (nTerm scons_q) [nHole; s; t].
+Definition var_zero_ := nTerm var_zero_q.
+Definition funcomp_ (f g: nterm) : nterm := nApp (nTerm funcomp_q) [nHole; nHole; nHole; f; g].
+Definition shift_ := nTerm shift_q.
+Definition id_ := nApp (nTerm id_q) [nHole].
+Definition up_ren_ren_ := nTerm up_ren_ren_q.
+
+Notation "g >>> f" := (funcomp_ f g) (at level 70, no associativity).
+
+
+(** Return a list of variable names for the input list of positions
+ ** [s0, s2, ..., sn-1] *)
+Definition getPattern {A: Type} (name: string) (l: list A) :=
+  mapi (fun i _ => name ++ string_of_nat i) l.
+
+
+(* Definition lambda_ (bname: string) (ty body: term) := *)
+(*   tLambda {| binder_name := nNamed bname; binder_relevance := Relevant |} ty body. *)
+
+Definition add_binders (bs: list (string * nterm)) (body: nterm) :=
+  List.fold_right (fun '(bname, btype) body => nLambda bname btype body) body bs.
+
+Definition add_tbinders (bs: list (string * nterm)) (body: nterm) :=
+  List.fold_right (fun '(bname, btype) body => nProd bname btype body) body bs.
+
+(** * The following definitions are just hardcoded for System F ty *)
+
+(** Create the argument type for the variable constructor of the given sort.
+ ** If we create well scoped code fin will be indexed by the element of the scope indices
+ ** corresponding to the sort.
+ ** For sort vl and ns = [nty; nvl], create fin nvl *)
+
+(* TODO make general *)
+Definition genVarArg (sort: string) : nterm := nat_.
+
+(** Construct the body of a definition depending on if the given sort matches the one in the binder *)
+Definition definitionBody (sort: tId) (binder: Binder) (singleMatch singleNoMatch: nterm) (* (f_listMatch: string -> tId -> term)  *) : nterm :=
+  match binder with
+  | Single sort' => if eqb sort sort'
+                   then singleMatch
+                   else singleNoMatch
+  (* TODO binder list case *)
+  (* | L.BinderList (p, sort') -> *)
+  (*   let (listMatch, listNoMatch) = f_listMatch p sort' in *)
+  (*   if sort = sort' then listMatch else listNoMatch *)
+  end.
+
+(** Extract the extra shifting argument from a BinderList.
+ ** In MetaCoq all binders are explicit so we don't even have the binvparameters function *)
+Definition bparameters (binder: Binder) : list term * list (term -> term) :=
+  match binder with
+  | Single x => ([], [])
+  (* | BinderList (m, _) -> ([ref_ m], [binder1_ ~implicit:true ~btype:nat_ m]) *)
+  end.
+
