src/quotes.v
@@ -1,8 +1,0 @@
-From MetaCoq.Template Require Import All.
-
-MetaCoq Quote Definition nat_q := nat.
-MetaCoq Quote Definition eq_q := @eq.
-MetaCoq Quote Definition eq_trans_q := @eq_trans.
-MetaCoq Quote Definition eq_refl_q := @eq_refl.
-MetaCoq Quote Definition f_equal_q := @f_equal.
-  
