src/tests/diverge.v
@@ -1,9 +1,12 @@
 (* tldr the finmap module from the coq stdlib constructs very large terms that will crash coq if you don't fully evaluate something like a G.mem_edge *)
+From ASUB Require Import hsig AL sigAnalyzer.
 Module diverge.
   From MetaCoq.Template Require Import All.
   Import MonadNotation.
   Inductive Id {A:Type} := IdC : A -> Id.
-  Require Import Arith.
+  Require Import Arith List String.
+  Open Scope string.
+  Import ListNotations.
 
   Definition mySigSpec : Spec := SFMap.fromList
                                    [  ("ty", [ {| con_parameters := [];
@@ -12,10 +15,10 @@ Module diverge.
                                                                    ; {| pos_binders := []; pos_head := Atom "ty" |} ] |}
                                                 ; {| con_parameters := [];
                                                      con_name := "all";
-                                                     con_positions := [ {| pos_binders := [ Single "ty" ]; pos_head := Atom "ty" |} ] |} ]) ].
+                                                     con_positions := [ {| pos_binders := [ Single "ty" ]; pos_head := Atom "ty" |} ] |} ]) 
 
-  Definition mySigSpec2 : Spec := SFMap.fromList
-                                   [  ("tm", [ {| con_parameters := [];
+  (* Definition mySigSpec2 : Spec := SFMap.fromList *)
+                                   ;  ("tm", [ {| con_parameters := [];
                                                    con_name := "app";
                                                    con_positions := [ {| pos_binders := []; pos_head := Atom "tm" |}
                                                                    ; {| pos_binders := []; pos_head := Atom "tm" |} ] |}
@@ -32,7 +35,7 @@ Module diverge.
      * Build graph, then check if edge exists two times while one expression is packed in some inductive type
      * WTF is happening here?
      * Feels like somehow state is handled wrongly since it works when I use a "fresh" copy of the graph for the second call to mem_edge *)
-    let spec := Hsig_example.mySigSpec2 in
+    let spec := mySigSpec in
     let g := build_graph spec in
     (* let g' := build_graph spec in *)
     let x1 := if G.mem_edge g "ty" "ty" then IdC (G.mem_edge g "ty" "ty") else IdC true in
@@ -43,7 +46,7 @@ Module diverge.
     (* let x1 := if G.mem_edge g "ty" "ty" then IdC (if G.mem_edge g "ty" "ty" then true else false) else IdC true in *)
     (* let x1 := if G.mem_edge g "vl" "vl" then IdC (g) else IdC g in *)
     (* Yannick: sollte man immer mal wieder tmeval all machen? *)
-    (* x2 <- tmEval hnf x1;; *)
+    (* x2 <- tmEval all x1;; *)
     match x1 with
     | IdC x => tmReturn x
     end.
