src/tests/printing.v
@@ -1,0 +1,19 @@
+(* Does MetaCoq already have facilities to pretty-print terms? *)
+From MetaCoq.Template Require Import All Pretty.
+Import String List.
+Import ListNotations.
+
+Check print_term.
+
+Definition foo := <% forall X:Type, X -> X %>.
+Print foo.
+
+(* yes it's possible. But it seems that if I want to use things from the environment like "eq" I need to set up the environment which is cumbersome *)
+Compute print_term ([], Monomorphic_ctx (LevelSet.Mkt [], ConstraintSet.Mkt [])) [] false foo.
+
+
+Definition bar := <% 0 = 0 %>.
+Compute print_term ([], Monomorphic_ctx (LevelSet.Mkt [], ConstraintSet.Mkt [])) [] false bar.
+
+
+
