src/tests/test.v
@@ -1,5 +1,15 @@
 From Coq Require Import String List.
-From MetaCoq.Template Require Import Ast Loader.
+From MetaCoq.Template Require Import All.
+MetaCoq Quote Definition nat_q := @eq.
+
+Require Import FunctionalExtensionality.
+Goal forall (x y: nat), x = y -> (fun z => z + x) = (fun z => z + y).
+Proof.
+  intros * H.
+  rewrite H.
+  reflexivity.
+Qed.
+
 Import ListNotations.
 Definition bAnon := {| binder_name := nAnon; binder_relevance := Relevant |}.
 Definition bNamed s := {| binder_name := nNamed s; binder_relevance := Relevant |}.
@@ -19,19 +29,45 @@ Qed.
 (** Evars *)
 MetaCoq Quote Definition lnil := @nil.
 MetaCoq Quote Definition listnat := (list nat).
+MetaCoq Quote Definition eq_q := @eq.
+MetaCoq Quote Definition zero_q := 0.
 MetaCoq Unquote Definition foo := (tCast (tApp lnil [hole]) Cast listnat).
 
 Local Open Scope string_scope.
 
 Goal list nat.
   (* Back and forth *)
-  let x := open_constr:(nil) in quote_term x (fun qt => 
-    ltac:(denote_term qt (fun unqt => set (e := eq_refl : unqt = x :> list bool)))).
+  (* Set Printing All. *)
+  let x := idtac in idtac x.
+  let x := open_constr:(cons 0 []) in quote_term x (fun qt =>
+    ltac:(idtac qt; (denote_term qt (fun unqt => idtac unqt; (set (e := eq_refl : unqt = x :> list _));
+                                    idtac unqt; idtac x));
+          idtac 0)).
     (* Creation of evars by denotation of 'hole' *)
+  Unset Printing Notations.
+  Set Printing All.
   let x := eval cbv in (tApp lnil [hole]) in
-  denote_term x (fun k => exact k).
+  denote_term x (fun k => idtac k; exact k).
 Defined.
 
+Lemma bla: Prop.
+  let x := constr:(tApp (tInd {| inductive_mind := (MPfile ["Logic"; "Init"; "Coq"], "eq"); inductive_ind := 0 |} []) [tEvar fresh_evar_id []; (tConstruct {| inductive_mind := (MPfile ["Datatypes"; "Init"; "Coq"], "nat"); inductive_ind := 0 |} 0 []); (tConstruct {| inductive_mind := (MPfile ["Datatypes"; "Init"; "Coq"], "nat"); inductive_ind := 0 |} 0 [])])
+  in idtac x; (denote_term x (fun unqt => idtac unqt; 
+                                       idtac x; exact unqt)).
+  
+  Unshelve.
+  (* the second seems to be the evar that is placed in eq but why do I even get the first? *)
+  exact Type. exact nat.
+Defined.
+
+(* ok so it does not really work above since I always get the shelved evars which I have to explicitly instantiate and below does not work either so I don't pursue this further. It would be an ugly hack anyways.
+
+ foo2 uses an Gallina-let and when I use x as an argument to denote_term it does not seem to reduce it (different semantics to ltac-let) which means that denote_term just sees x. No idea how to reduce it though *)
+Fail Definition foo2 : term :=
+  let x := (tApp (tInd {| inductive_mind := (MPfile ["Logic"; "Init"; "Coq"], "eq"); inductive_ind := 0 |} []) [tEvar fresh_evar_id []; (tConstruct {| inductive_mind := (MPfile ["Datatypes"; "Init"; "Coq"], "nat"); inductive_ind := 0 |} 0 []); (tConstruct {| inductive_mind := (MPfile ["Datatypes"; "Init"; "Coq"], "nat"); inductive_ind := 0 |} 0 [])])
+  in ltac:(denote_term x (fun unqt => idtac unqt; 
+                                    idtac unqt; exact unqt)).
+    
 Goal True.
   let x := eval cbv in (tLambda bAnon listnat hole) in
   (* We check that created evars are in the right context *)
